More work on CPS. Identify some framework improvements

src/named/CPS.v
@@ -8,7 +8,7 @@ Set Bullet Behavior "Strict Subproofs".
 From Ltac2 Require Import Ltac2.
 Set Default Proof Mode "Classic".
 From Utils Require Import Utils.
-From Named Require Import IExp IRule ICore Subst STLC.
+From Named Require Import IExp IRule ICore ICompilers Subst STLC.
 Require Import String.
 
 
@@ -36,38 +36,109 @@ Instance elab_stlc_bot_inst : Elaborated stlc_bot :=
   elab_pf := elab_stlc_bot_pf;
   }.
 
+(* equivalent definition
+Definition lookup_args l n :=
+  get_rule_args ( named_list_lookup (ARule.sort_rule [::] [::]) l n).
+Definition id_compiler l :=
+  make_compiler (fun c s => scon c (map var (lookup_args l c)))
+                (fun c s => con c (map var (lookup_args l c)))
+                (strip_args l).
+*)
 
-From Named Require Import Compilers.
-  
-Fixpoint make_compiler
-           (cmp_sort : string -> list string -> Exp.sort)
-           (cmp_exp : string -> list string -> Exp.exp)
-           (l : Rule.lang) : compiler :=
+Fixpoint id_compiler (l : ARule.lang) : compiler :=
   match l with
-  | (n,Rule.sort_rule c)::l' =>
-    (n,sort_case (map fst c) (cmp_sort n (map fst c)))
-      ::(make_compiler cmp_sort cmp_exp l')
-  | (n,Rule.term_rule c _)::l' => (n,term_case (map fst c) (cmp_exp n (map fst c)))
-      ::(make_compiler cmp_sort cmp_exp l')
-  | (n,_)::l' => 
-    (make_compiler cmp_sort cmp_exp l')
+  | (n,ARule.sort_rule c args)::l' =>
+    (n,sort_case (map fst c) (scon n (map var args)))
+      ::(id_compiler l')
+  | (n,ARule.term_rule c args _)::l' =>
+    (n,term_case (map fst c) (con n (map var args)))
+      ::(id_compiler l')
+  | (n,_)::l' => id_compiler l'
   | [::] => [::]
   end.
 
+Fixpoint eid_compiler (l : ARule.lang) : Compilers.compiler :=
+  match l with
+  | (n,ARule.sort_rule c args)::l' =>
+    (n,Compilers.sort_case (map fst c) (Exp.srt n (map Exp.var (map fst c))))
+      ::(eid_compiler l')
+  | (n,ARule.term_rule c args _)::l' =>
+    (n,Compilers.term_case (map fst c) (Exp.con n (map Exp.var (map fst c))))
+      ::(eid_compiler l')
+  | (n,_)::l' => eid_compiler l'
+  | [::] => [::]
+  end.
 
-Definition id_compiler :=
-  make_compiler (fun c s => Exp.srt c (map Exp.var s))
-                (fun c s => Exp.con c (map Exp.var s)).
-
+(* TODO: generalize id compiler 
 (* TODO: prove *) 
-Lemma preserving_compiler_embed p lt cmp ls
-  : preserving_compiler lt cmp ls ->
-    preserving_compiler (p::lt) cmp ls.
+Lemma preserving_compiler_embed n r lt cmp ls
+  : Core.fresh n lt ->
+    Compilers.preserving_compiler lt cmp ls ->
+    Compilers.preserving_compiler ((n,r)::lt) cmp ls.
+Proof.
+Admitted.
+
+Lemma elab_preserving_compiler_embed n r lt cmp ecmp ls
+  : Core.fresh n lt ->
+    elab_preserving_compiler lt cmp ecmp ls ->
+    elab_preserving_compiler ((n,r)::lt) cmp ecmp ls.
+Proof.
+Admitted.
+
+Lemma fresh_strip_args
+  : forall (l : named_list ARule.rule) (name : Exp.str_eqType),
+       Core.fresh name (strip_args l) -> Core.fresh name l.
 Proof.
 Admitted.
 
 Lemma preserving_id_compiler l
-  : Core.wf_lang l -> preserving_compiler l (id_compiler l) l.
+  : Core.wf_lang (strip_args l) -> elab_preserving_compiler l (id_compiler l) (eid_compiler l) l.
+Proof.
+  elim l; simpl; intros.
+  { constructor. }
+  {
+    destruct a.
+    simpl in *.
+    destruct r; simpl in *; inversion H0; subst; constructor;
+      eauto using elab_preserving_compiler_embed, fresh_strip_args.
+    {
+      eapply elab_sort_by'; simpl; rewrite eqb_refl; simpl; eauto.
+      admit.
+      {
+        elim l1; cbn.
+        {
+          inversion H6; subst.
+          revert H2.
+          elim c; cbn.
+          { constructor. }
+          { intros.
+            destruct a; cbn.
+            inversion H2; subst.
+            repeat(cbn; step_elab()); auto.
+            inversion
+            cbn.
+      Search  _ (map _ (map _ _)).
+      apply strip_args_fresh.
+      Search strip_args.
+    {
+      
+      
+    split.
+
+Derive elab_id_compiler
+       SuchThat (forall lt ls, elab_preserving_compiler lt (id_compiler ls) (elab_id_compiler ls) ls)
+       As elab_id_compiler_pf.
+Proof.
+  assert (exists b, elab_id_compiler = fun l => b l).
+  eexists; cbv; reflexivity.
+  destruct H as [eidc H].
+  rewrite H.
+  intros lt ls.
+  induction ls.
+  { cbn. constructor. }
+
+Lemma preserving_id_compiler l
+  : Core.wf_lang l -> elab_preserving_compiler l (id_compiler l) l.
 Proof.
   elim l > [constructor|].
   intros p l'.
@@ -80,9 +151,7 @@ Proof.
     ltac1:(instantiate (1:=c)).
     admit.
     
-  
-(*Definition to_cmp l c' : compiler :=
-  map c' (map fst l).*)
+*)
 
 (*
 Definition twkn g a b := {{#"ty_subst"(#"ext"(g,a),g,#"wkn"(g,a),b)}}.
@@ -109,11 +178,14 @@ Definition double_neg t :=
 
 Definition lam e := {{e #"lambda" !e}}.
 
-Definition cps_sort (c:string) args : sort := srt c (map Exp.var args).
-Definition cps (c : string) args : exp :=
+Definition lookup_args l n :=
+  get_rule_args ( named_list_lookup (ARule.sort_rule [::] [::]) l n).
+
+Definition cps_sort (c:string) args : sort := scon c (map var args).
+Definition cps (c : string) (args : list string) : exp :=
   match c, args with
   | "->", [:: B; A; G] =>
-    double_neg {{e #"->" !A !B}}
+    double_neg {{e #"->" %A %B}}
   | "lambda", [:: e; B; A; G] =>
     ret_val {{e #"lambda" %e}}
   | "app", [:: e2; e1; b; a; g] =>
@@ -121,9 +193,150 @@ Definition cps (c : string) args : exp :=
     let x1 := wkn_n 1 {{e #"hd"}} in
     let x2 := {{e #"hd"}} in
     lam
-      (let_bind (wkn_n 1 e1)
-      (let_bind (wkn_n 2 e2)
-      {{e #"app" %k (#"app" %x1 %x2)}}))
-  | _,_ => con c args
+      (let_bind (wkn_n 1 (var e1))
+      (let_bind (wkn_n 2 (var e2))
+      {{e #"app" !k (#"app" !x1 !x2)}}))
+  | _,_ => con c (map var (lookup_args elab_stlc c))
   end%string.
 
+Derive elab_cps
+       SuchThat (elab_preserving_compiler elab_stlc_bot (make_compiler cps_sort cps (strip_args elab_stlc)) elab_cps elab_stlc)
+       As elab_cps_pf.
+Proof.
+  simpl.
+  repeat (match! goal with
+  | [ |-  elab_preserving_compiler _ ((_,sort_case _ _)::_) _ _]=>
+    apply preserving_compiler_sort'
+  | [ |-  elab_preserving_compiler _ ((_,term_case _ _)::_) _ _]=>
+    apply preserving_compiler_term'
+  | [ |-  elab_preserving_compiler _ _ _ _]=>
+    constructor
+  | [|-_] => simpl; step_elab()
+          end).
+  solve [apply elab_term_by'; repeat (simpl;step_elab())].
+  solve [apply elab_term_by'; repeat (cbn;step_elab())].
+  {
+    cbn.
+    eapply (Core.le_term_by' "id_right"%string);repeat(cbn; step_elab()); reflexivity.
+  }    
+  {
+    cbn.
+    eapply (Core.le_term_by' "id_left"%string);repeat(cbn; step_elab()); reflexivity.
+  }   
+  {
+    cbn.
+    eapply (Core.le_term_by' "cmp_assoc"%string);repeat(cbn; step_elab()); reflexivity.
+  } 
+  solve [apply elab_term_by'; repeat (cbn;step_elab())].
+  solve [step_elab()].
+  solve [apply elab_term_by'; repeat (cbn;step_elab())].
+  {
+    cbn.
+    eapply (Core.le_term_by' "ty_subst_id"%string);repeat(cbn; step_elab()); reflexivity.
+  }   
+  {
+    cbn.
+    eapply (Core.le_term_by' "ty_subst_cmp"%string);repeat(cbn; step_elab()); reflexivity.
+  }   
+  {
+    cbn.
+    eapply (Core.le_term_by' "el_subst_id"%string);repeat(cbn; step_elab()); reflexivity.
+  }   
+  {
+    cbn.
+    eapply (Core.le_term_by' "el_subst_cmp"%string);repeat(cbn; step_elab()); reflexivity.
+  }   
+  solve [apply elab_term_by'; repeat (cbn;step_elab())].
+  solve [apply elab_term_by'; repeat (cbn;step_elab())].
+  {
+    cbn.
+    eapply (Core.le_term_by' "cmp_forget"%string);repeat(cbn; step_elab()); reflexivity.
+  }   
+  {
+    cbn.
+    eapply (Core.le_term_by' "id_emp_forget"%string);repeat(cbn; step_elab()); reflexivity.
+  }   
+  solve [apply elab_term_by'; repeat (cbn;step_elab())].
+  {
+    cbn.
+    apply elab_term_by'; repeat (cbn;step_elab()).
+    apply Core.wf_term_by'; repeat (cbn;step_elab()).
+  }
+  solve [apply elab_term_by'; repeat (cbn;step_elab())].
+  solve [apply elab_term_by'; repeat (cbn;step_elab())].
+  {
+    cbn.
+    eapply (Core.le_term_by' "wkn_snoc"%string);repeat(cbn; step_elab()); reflexivity.
+  }   
+  {
+    cbn.
+    eapply (Core.le_term_by' "snoc_hd"%string);repeat(cbn; step_elab()); reflexivity.
+  }   
+  {
+    cbn.
+    eapply (Core.le_term_by' "cmp_snoc"%string);repeat(cbn; step_elab()); reflexivity.
+  }   
+  {
+    cbn.
+    eapply (Core.le_term_by' "snoc_wkn_hd"%string);repeat(cbn; step_elab()); reflexivity.
+  }
+  (* end of subst lang *)
+  {
+    cbn.
+    repeat (apply elab_term_by'; repeat (cbn;step_elab())).
+  }
+  {
+    cbn.
+    apply elab_term_by'; repeat (cbn;step_elab()).
+    apply elab_term_by'; repeat (cbn;step_elab()).
+    apply elab_term_by'; repeat (cbn;step_elab()).
+    apply elab_term_by'; repeat (cbn;step_elab()).
+    cbn.
+    Require Import Named.Recognizers.
+    apply Core.wf_term_by'; repeat (cbn;step_elab()).
+    apply Core.wf_term_by'; repeat (cbn;step_elab()).
+    apply Core.wf_term_by'; repeat (cbn;step_elab()).
+    apply Core.wf_term_by'; repeat (cbn;step_elab()). 
+    apply elab_term_by'; repeat (cbn;step_elab()).
+    apply elab_term_by'; repeat (cbn;step_elab()).
+    apply elab_term_by'; repeat (cbn;step_elab()).
+    apply elab_term_by'; repeat (cbn;step_elab()).
+    apply elab_term_by'; repeat (cbn;step_elab()).
+    repeat (cbn;step_elab()).
+    apply elab_term_by'; repeat (cbn;step_elab()).
+    apply elab_term_by'; repeat (cbn;step_elab()).
+    apply elab_term_by'; repeat (cbn;step_elab()).
+    apply elab_term_by'; repeat (cbn;step_elab()).
+    apply elab_term_by'; repeat (cbn;step_elab()).
+    cbn. TODO: apply ty_subst conversion
+    apply elab_term_by'; repeat (cbn;step_elab()).
+    apply elab_term_by'; repeat (cbn;step_elab()).
+    apply elab_term_by'; repeat (cbn;step_elab()).
+    apply elab_term_by'; repeat (cbn;step_elab()).
+    apply elab_term_by'; repeat (cbn;step_elab()).
+  }
+  solve [apply elab_term_by'; repeat (cbn;step_elab())].
+  solve [apply elab_term_by'; repeat (cbn;step_elab())].
+  solve [apply elab_term_by'; repeat (cbn;step_elab())].
+  solve [apply elab_term_by'; repeat (cbn;step_elab())].
+  solve [apply elab_term_by'; repeat (cbn;step_elab())].
+  solve [apply elab_term_by'; repeat (cbn;step_elab())].
+  solve [apply elab_term_by'; repeat (cbn;step_elab())].
+  solve [apply elab_term_by'; repeat (cbn;step_elab())].
+  solve [apply elab_term_by'; repeat (cbn;step_elab())].
+  unfold elaboration.
+  unfold elab_cat_lang_inst.
+  unfold elab_cat_lang.
+  repeat (match! goal with
+  | [ |-  elab_preserving_compiler _ ((_,term_case _ _)::_) _ _]=>
+    apply preserving_compiler_term'
+  | [ |-  elab_preserving_compiler _ _ _ _]=>
+    constructor
+  | [|-_] => cbn; step_elab()
+          end).
+
+  apply preserving_compiler_term'; 
+  cbv.
+  TODO: friendly construxtors to figure out the issues?
+  constructor.
+  repeat constructor.
