README.md
@@ -1,10 +1,5 @@
-#Candidate changes:
-
-* make datatype(s?) w/ language, ctx as a parameter, presuppositions as args, prove eq
-
 #TODOs
 
-* fix various warnings (e.g. hint database)
-* make library of better induction schemes
+* determine whether wf_sort wanted in wf_args_cons constructor
+* determine whether there is an issue w/ current lax typing on le judgments
 * prune obsolete lemmas
-* determine minimal presuppositions needed in proof tree 
